NuLLReps.thy
@@ -745,29 +745,6 @@ lemma [\<nu>intro]: "\<nu>Ownership (MemMap N) ownership"
   unfolding \<nu>Ownership_def by (simp add: owning_forall memcon_forall memptr_forall object_exists)
 lemma [\<nu>intro]: "\<nu>Zero (MemMap N) \<down_fish_tail>" unfolding \<nu>Zero_def by simp
 
-subsection \<open>\<nu>-abstraction : Slice\<close>
-
-definition MemSlice :: "(('a::field), 'b) nu \<Rightarrow> ('a memobj, 'b list object owning) nu"
-  where "MemSlice N p x = (
-    case (p,x) of (zp \<left_fish_tail> memcon f , z \<left_fish_tail> ((seg |+ ofs) \<R_arr_tail> x)) \<Rightarrow>
-        (zp = z) \<and> (\<forall>i < length x. \<exists>p'. f (seg |+ (ofs + int i)) = Some p' \<and> (p' \<nuLinkL> N \<nuLinkR> x ! i) )
-    | (\<down_fish_tail> , \<down_fish_tail>) \<Rightarrow> True | _ \<Rightarrow> False)"
-
-lemma [simp]: "zp \<left_fish_tail> memcon f \<nuLinkL> MemSlice N \<nuLinkR> z \<left_fish_tail> (seg |+ ofs) \<R_arr_tail> x \<longleftrightarrow>
-    (zp = z) \<and> (\<forall>i < length x. \<exists>p'. f (seg |+ (ofs + int i)) = Some p' \<and> (p' \<nuLinkL> N \<nuLinkR> x ! i) )"
-  and [simp]: "\<down_fish_tail> \<nuLinkL> MemSlice N \<nuLinkR> x' \<longleftrightarrow> x' = \<down_fish_tail>" and [simp]: "p' \<nuLinkL> MemSlice N \<nuLinkR> \<down_fish_tail> \<longleftrightarrow> p' = \<down_fish_tail>"
-  unfolding MemSlice_def Refining_ex by (auto simp add: memptr_forall split: memcon.split owning.split)
-
-lemma [elim,\<nu>elim]: "z \<left_fish_tail> a \<R_arr_tail> xs \<ratio> MemSlice N \<Longrightarrow>
-    ((\<And>i. i < length xs \<Longrightarrow> xs ! i \<ratio> N) \<Longrightarrow> C) \<Longrightarrow> C"
-  unfolding Inhabited_def by (cases a; auto 6 6 simp add: lrep_exps list_all2_conv_all_nth) 
-
-lemma [\<nu>intro]: "\<nu>Share (MemSlice N) (\<lambda>x. True) share"
-  unfolding \<nu>Share_def by (simp add: lrep_exps)
-lemma [\<nu>intro]: "\<nu>Disposable \<tort_lbrace>\<down_fish_tail> \<tycolon> MemSlice N\<tort_rbrace>" unfolding \<nu>Disposable_def by simp
-lemma [\<nu>intro]: "\<nu>CEqual (MemSlice N) (\<lambda>x y. True) (\<lambda>x y. True)" unfolding \<nu>CEqual_def by simp
-lemma [\<nu>intro]: "\<nu>Zero (MemSlice N) \<down_fish_tail>" unfolding \<nu>Zero_def by simp
-
 section \<open>Ghost\<close>
 
 datatype 'a ghost = ghost 'a
